examples/ghc/theories/CoreSubst.v
@@ -1167,6 +1167,7 @@ Proof.
        auto.
 Qed.
 
+
 Lemma substExpr_ok : forall e s vs in_scope_set env u0 u1, 
     WellScoped_Subst (Mk_Subst in_scope_set env u0 u1) vs -> 
     WellScoped e vs -> 
@@ -1410,8 +1411,10 @@ Proof.
     rewrite -> extendVarSetList_nil in *.
     eapply StrongSubset_extendVarSetList.
     eauto.
-  - intros.
+  - move => tickish e0 IH s vs in_scope_set env u1 u2 WSS WST.
     hs_simpl.
-    unfold WellScoped in *. fold WellScoped in *.
-    eapply H; eauto.
+    simpl in WST.
+    move: WST => [WSe ?].
+    unfold CoreUtils.mkTick.
+    eapply IH; eauto.
 Qed.
