examples/ghc/theories/Exitify.v
@@ -3175,8 +3175,9 @@ Next Obligation.
     assumption.
   * (* Tick *)
     simpl in *.
+    destruct HWS as [HWS HWT].
     epose proof (IH _ _ _ _ _ HWS HJPV ltac:(solve_subVarSet)).
-    assumption.
+    intuition.
   * (* Type *)
     intuition.
   * (* Coercion *)
